proof/Main.v
@@ -6,23 +6,6 @@ Require Import Ty.
 Require Import Context.
 
 (* evaluation *********************************************)
-Inductive STEP : exp -> exp -> Prop := 
-  | EVAppAbs 
-    :   forall x T t12 v2 
-    ,   VALUE v2 
-    ->  STEP  (XApp (XLam x T t12) v2)
-              (subst x v2 t12)
-
-  | EVApp1 
-    :   forall t1 t1' t2
-    ,   STEP t1 t1'
-    ->  STEP (XApp t1 t2) (XApp t1' t2)
-
-  | EVApp2
-    :   forall v1 t2 t2'
-    ,   VALUE v1
-    ->  STEP  t2 t2'
-    ->  STEP  (XApp v1 t2) (XApp v1 t2').
 
 
 Hint Constructors STEP.
