proof/EvJudge.v
@@ -1,0 +1,20 @@
+
+Require Export Exp.
+
+Inductive STEP : exp -> exp -> Prop := 
+  | EVAppAbs 
+    :   forall x T t12 v2 
+    ,   VALUE v2 
+    ->  STEP  (XApp (XLam x T t12) v2)
+              (subst x v2 t12)
+
+  | EVApp1 
+    :   forall t1 t1' t2
+    ,   STEP t1 t1'
+    ->  STEP (XApp t1 t2) (XApp t1' t2)
+
+  | EVApp2
+    :   forall v1 t2 t2'
+    ,   VALUE v1
+    ->  STEP  t2 t2'
+    ->  STEP  (XApp v1 t2) (XApp v1 t2').
