proof/Progress.v
@@ -1,0 +1,35 @@
+
+Require Import TyJudge.
+Require Import EvJudge.
+
+
+Theorem progress
+ :  forall t T
+ ,  TYPE  empty t T
+ -> VALUE t \/ (exists t', STEP t t').
+Proof.
+ intros t T. intros Ht.
+ remember (@empty ty) as G.
+ induction Ht.
+ Case "XVar".
+  left. subst. inversion H.
+ Case "XLam".
+  left. auto.
+ Case "XApp".
+  right.
+  destruct IHHt1. auto. 
+  SCase "t1 value".
+   destruct H. destruct IHHt2. trivial.
+   SSCase "t2 value".
+    exists (subst x t2 t). apply EVAppAbs. trivial.
+   SSCase "t2 steps".
+    destruct H as [t2' Htsp].
+    exists (XApp (XLam x T t) t2').
+    apply EVApp2. trivial. trivial.
+  SCase "t1 steps".
+   destruct H as [t1' Htsp].
+   exists (XApp t1' t2).
+   apply EVApp1. trivial.
+Qed.
+
+
